ram-linear-time/concepts/Lax11.lean
@@ -1,3 +1,7 @@
 import Lax11.GraphEncoding
 import Lax11.ConnectedComponents
+import Lax11.Mso
+import Lax11.CliqueExpr
+import Lax11.InstanceEncoding
+import Lax11.Courcelle
 import Lax11.VertexCover
